\documentclass{article}

\begin{document}

\section{Aufgabe 1}

\begin{tabular}{| c | l | l |}
    \hline
    Nr. & Rekursion & Polynom \\\hline
    1 & $s_n = s_{n-3} + s_{n-1}$ & $f(X) = X^3 - X^2 - 1$\\\hline
    2 & $s_n = s_{n-3} + s_{n-1}$ & $f(X) = X^4 - X^3 - X$\\\hline
    3 & $s_n = s_{n-5} + s_{n-4} + s_{n-3} + s_{n-1}$ & $f(X) = X^5 - X^4 - X^2 - X - 1$\\\hline
\end{tabular}

\section{Aufgabe 2}

\begin{enumerate}
    \item $x^2 + 1 = (x+1)^2$
    \item $x^3 + 1 = (x+1)(x^2 + x + 1)$
    \item $x^4 + x^2 + 1 = (x^2 + x + 1)^2$
\end{enumerate}

\section{Aufgabe 3}

\begin{tabular}{| l | l |}
    \hline
    Polynom & Rekursion \\\hline
    $f(X) = X^5 + X^4 + X^2 + X + 1$ & $s_{n+5} = s_{n+4} + s_{n+2} + s_{n+1} + s_{n}$\\\hline
    $f(X) = X^5 + X^4 + X^3 + X + 1$ & $s_{n+5} = s_{n+4} + s_{n+3} + s_{n+1} + s_{n}$\\\hline
\end{tabular}

\section{Aufgabe 4}

Rückkopplungspolynom: $f(X) = X^5 + X + 1 = (X^3 - X^2 + 1)(X^2 + X + 1)$

\section{Aufgabe 6}

\subsection{}

Outputfolge: \textbf{00001 00011}

00001 -> 0: $c_4 = 0$\\
00010 -> 0: $c_3 = 0$\\
00100 -> 0: $c_2 = 0$\\
01000 -> 1: $c_1 = 1$\\
10001 -> 1: $c_0 + c_4 = 1 \implies c_0 = 1$\\

Schieberegister: $c = 00011$

\subsection{}

110 000 100 000 11: geht nicht\\
1100 0010 0000 11: geht nicht\\
11000 01000 0011: geht nicht\\
110000 100000 11: möglich\\

\subsection{}

0000 -> 1000: unmöglich
\end{document}
